theories/Match.v
@@ -1,4 +1,6 @@
 From LinearCore Require
+  BoundIn
+  Context
   Map
   Pattern
   Term
@@ -9,91 +11,345 @@ From LinearCore Require Import
 
 
 
-Inductive Strict : Pattern.strict -> Term.term -> Map.to Term.term -> Prop :=
-  | Ctr matches (E : Map.Empty matches) ctor
-      : Strict (Pattern.Ctr ctor) (Term.Ctr ctor) matches
-  | App
-      function_pattern function function_matches (function_matched : Strict function_pattern function function_matches)
-      argument_name (N : forall (I : Map.In function_matches argument_name), False)
+Inductive Strict (context : Context.context) : Pattern.strict -> Term.term -> Context.context -> Prop :=
+  | Ctr context_with_matches (E : Map.Eq context context_with_matches) ctor
+      : Strict context (Pattern.Ctr ctor) (Term.Ctr ctor) context_with_matches
+  | App function_pattern function
+      context_with_function_matches (function_matched :
+        Strict context function_pattern function context_with_function_matches)
+      argument_name (N : forall (I : Map.In context_with_function_matches argument_name), False)
       (* can't match the same name twice in the same pattern ^^^ *)
-      argument matches (A : Map.Add argument_name argument function_matches matches)
-      : Strict (Pattern.App function_pattern argument_name) (Term.App function argument) matches
+      argument context_with_matches (A :
+        Map.Add argument_name argument context_with_function_matches context_with_matches)
+      : Strict context (Pattern.App function_pattern argument_name) (Term.App function argument) context_with_matches
   .
-Arguments Strict strict term matches.
+Arguments Strict context strict term context_with_matches.
 
-Fixpoint strict pattern term : option (Map.to Term.term) :=
+Fixpoint strict context pattern term : option Context.context :=
   match pattern, term with
   | Pattern.Ctr constructor_pattern, Term.Ctr constructor =>
-      if Constructor.eq constructor_pattern constructor then Some Map.empty else None
+      if Constructor.eq constructor_pattern constructor then Some context else None
   | Pattern.App function_pattern argument_name, Term.App function argument =>
-      match strict function_pattern function with None => None | Some function_matches =>
-        Map.disjoint_add argument_name argument function_matches
+      match strict context function_pattern function with
+      | None => None
+      | Some context_with_function_matches =>
+          Map.disjoint_add argument_name argument context_with_function_matches
       end
   | _, _ => None
   end.
 
-Lemma strict_det pattern term
-  matches1 (S1 : Strict pattern term matches1)
-  matches2 (S2 : Strict pattern term matches2)
-  : Map.Eq matches1 matches2.
+Lemma strict_det
+  c1 p1 t1 m1 (S1 : Strict c1 p1 t1 m1)
+  c2 (Ec : Map.Eq c1 c2)
+  p2 (Ep : p1 = p2)
+  t2 (Et : t1 = t2)
+  m2 (S2 : Strict c2 p2 t2 m2)
+  : Map.Eq m1 m2.
 Proof.
-  generalize dependent matches2. induction S1; intros; invert S2.
-  - split; intro F; [contradiction (E k) | contradiction (E0 k)]; eexists; eassumption.
-  - eapply Map.add_det; [exact A | reflexivity | reflexivity | apply Map.eq_refl |].
-    eapply Map.add_eq; [exact A0 | reflexivity | reflexivity |].
-    apply Map.eq_sym. apply IHS1. exact function_matched.
+  subst. generalize dependent m2. induction S1; intros; invert S2.
+  - eapply Map.eq_trans. { apply Map.eq_sym. eassumption. } eapply Map.eq_trans; eassumption.
+  - eapply Map.add_det; try reflexivity; try eassumption. apply IHS1. exact function_matched.
 Qed.
 
-Lemma strict_spec pattern term
-  : Reflect.Option (Strict pattern term) (strict pattern term).
+Lemma strict_spec context pattern term
+  : Reflect.Option (Strict context pattern term) (strict context pattern term).
 Proof.
   generalize dependent term. induction pattern; intros;
   destruct term; try solve [constructor; intros t C; invert C].
   - unfold strict. destruct (Constructor.eq_spec constructor constructor0); constructor.
-    + subst. constructor. apply Map.empty_empty.
+    + subst. constructor. apply Map.eq_refl.
     + intros t C. invert C. apply N. reflexivity.
-
-  - (* See if the curried constructor matched successfully: *)
-    simpl strict. destruct (IHpattern term1) as [function_matches function_matched | N]. 2: {
+  - simpl strict. destruct (IHpattern term1) as [function_matches function_matched | N]. 2: {
       constructor. intros t C. invert C. apply N in function_matched as []. }
-
-    (* See if `argument` was already in `function_matches` (i.e. duplicated, i.e. bad) *)
     destruct (Map.find_spec function_matches argument) as [duplicated F | N]. 2: {
       constructor. econstructor. { eassumption. } { intros [y F]. apply N in F as []. }
       apply Map.add_overriding. cbn. intros. apply N in F as []. }
-    constructor. intros t C. invert C. apply N; clear N. eexists. eapply strict_det; [| | eassumption]; eassumption.
+    constructor. intros t C. invert C. apply N; clear N. eexists.
+    eapply strict_det; try reflexivity; [eassumption | | | eassumption];
+    try eassumption. apply Map.eq_refl.
+Qed.
+
+Lemma in_strict {context strict term context_with_matches} (S : Strict context strict term context_with_matches) x
+  : Map.In context_with_matches x <-> (BoundIn.Strict strict x \/ Map.In context x).
+Proof.
+  generalize dependent x. induction S; intros.
+  - erewrite Map.in_eq. 2: { apply Map.eq_sym. exact E. }
+    split. { intro I. right. exact I. } intros [B | I]. { invert B. } exact I.
+  - split.
+    + intros [y F]. apply A in F as [[-> ->] | F]. { left. left. }
+      eassert (I : Map.In _ _). { eexists. exact F. }
+      apply IHS in I as [B | I]; [left | right]. { right. exact B. } exact I.
+    + intro I. eapply Map.in_add. { eassumption. }
+      destruct I as [B | I]; [invert B; [left; reflexivity |] |];
+      right; apply IHS; [left | right]; assumption.
 Qed.
 
 
 
-(* TODO: match a reference. requires context. *)
+Inductive StrictRef (context : Context.context) : Pattern.strict -> Term.term -> Term.term -> Context.context -> Prop :=
+  | CtrR context_with_matches (E : Map.Eq context context_with_matches) ctor
+      : StrictRef context (Pattern.Ctr ctor) (Term.Ctr ctor) (Term.Ctr ctor) context_with_matches
+  | AppR
+      function_pattern function context_with_function_matches function_cleaved (function_matched :
+        StrictRef context function_pattern function function_cleaved context_with_function_matches)
+      argument_name (N : forall (I : Map.In context_with_function_matches argument_name), False)
+      (* can't match the same name twice in the same pattern ^^^ *)
+      argument context_with_matches (A :
+        Map.Add argument_name argument context_with_function_matches context_with_matches)
+      : StrictRef context
+        (Pattern.App function_pattern argument_name)
+        (Term.App function argument)
+        (Term.App function_cleaved (Term.Mov argument_name))
+        context_with_matches
+  .
+Arguments StrictRef context strict term cleaved context_with_matches.
+
+Fixpoint strict_ref context pattern term : option (Term.term * Context.context) :=
+  match pattern, term with
+  | Pattern.Ctr constructor_pattern, Term.Ctr constructor =>
+      if Constructor.eq constructor_pattern constructor then Some (Term.Ctr constructor, context) else None
+  | Pattern.App function_pattern argument_name, Term.App function argument =>
+      match strict_ref context function_pattern function with
+      | None => None
+      | Some (function_cleaved, context_with_function_matches) =>
+          match Map.disjoint_add argument_name argument context_with_function_matches with
+          | None => None
+          | Some context_with_matches =>
+              Some (Term.App function_cleaved (Term.Mov argument_name), context_with_matches)
+          end
+      end
+  | _, _ => None
+  end.
+
+Lemma strict_ref_det
+  {c1 p1 t1 y1 m1} (S1 : StrictRef c1 p1 t1 y1 m1)
+  {c2} (Ec : Map.Eq c1 c2)
+  {p2} (Ep : p1 = p2)
+  {t2} (Et : t1 = t2)
+  {y2 m2} (S2 : StrictRef c2 p2 t2 y2 m2)
+  : y1 = y2 /\ Map.Eq m1 m2.
+Proof.
+  subst. generalize dependent m2. generalize dependent y2. induction S1; intros; invert S2.
+  - split. { reflexivity. } eapply Map.eq_trans. { apply Map.eq_sym. eassumption. } eapply Map.eq_trans; eassumption.
+  - specialize (IHS1 _ _ function_matched) as [<- IH]. split. { reflexivity. }
+    eapply Map.add_det; try reflexivity; eassumption.
+Qed.
+
+Lemma strict_ref_spec context pattern term
+  : Reflect.Option (fun pair => StrictRef context pattern term (fst pair) (snd pair)) (strict_ref context pattern term).
+Proof.
+  generalize dependent term. induction pattern; intros;
+  destruct term; try solve [constructor; intros t C; invert C].
+  - unfold strict_ref. destruct (Constructor.eq_spec constructor constructor0); constructor.
+    + subst. constructor. apply Map.eq_refl.
+    + intros t C. invert C. apply N. reflexivity.
+  - simpl strict_ref. destruct (IHpattern term1) as [[cleaved function_matches] function_matched | N]. 2: {
+      constructor. intros t C. invert C. apply (N (_, _)) in function_matched as []. }
+    destruct (Map.find_spec function_matches argument) as [duplicated F | N]. 2: {
+      constructor. econstructor. { eassumption. } { intros [y F]. apply N in F as []. }
+      apply Map.add_overriding. cbn. intros. apply N in F as []. }
+    constructor. intros t C. invert C. apply N; clear N. eexists.
+    eapply strict_ref_det; try reflexivity; [eassumption | | | eassumption];
+    try eassumption. apply Map.eq_refl.
+Qed.
+
+Lemma in_strict_ref {context strict term cleaved context_with_matches}
+  (S : StrictRef context strict term cleaved context_with_matches) x
+  : Map.In context_with_matches x <-> (BoundIn.Strict strict x \/ Map.In context x).
+Proof.
+  generalize dependent x. induction S; intros.
+  - erewrite Map.in_eq. 2: { apply Map.eq_sym. exact E. }
+    split. { intro I. right. exact I. } intros [B | I]. { invert B. } exact I.
+  - split.
+    + intros [y F]. apply A in F as [[-> ->] | F]. { left. left. }
+      eassert (I : Map.In _ _). { eexists. exact F. }
+      apply IHS in I as [B | I]; [left | right]. { right. exact B. } exact I.
+    + intro I. eapply Map.in_add. { eassumption. }
+      destruct I as [B | I]; [invert B; [left; reflexivity |] |];
+      right; apply IHS; [left | right]; assumption.
+Qed.
 
 
 
-(*Variant Pattern : Pattern.pattern -> Term.term -> Map.to Term.term -> Prop :=*)
-(*  | Nam name term matches (S : Map.Singleton name term matches)*)
-(*      : Pattern (Pattern.Nam name) term matches*)
-(*  | Pat strict term matches (strict_matched : Strict strict term matches)*)
-(*      : Pattern (Pattern.Pat strict) term matches*)
-(*  .*)
-(*Arguments Pattern pattern term matches.*)
-(**)
-(*Definition pattern patt term :=*)
-(*  match patt with*)
-(*  | Pattern.Nam name => Some (Map.singleton name term)*)
-(*  | Pattern.Pat s => strict s term*)
-(*  end.*)
-(**)
-(*Lemma pattern_det patt term*)
-(*  matches1 (S1 : Pattern patt term matches1)*)
-(*  matches2 (S2 : Pattern patt term matches2)*)
-(*  : Map.Eq matches1 matches2.*)
-(*Proof. invert S1; invert S2. { eapply Map.singleton_det; eassumption. } eapply strict_det; eassumption. Qed.*)
-(**)
-(*Lemma pattern_spec patt term*)
-(*  : Reflect.Option (Pattern patt term) (pattern patt term).*)
-(*Proof.*)
-(*  destruct patt; cbn. { constructor. constructor. apply Map.singleton_singleton. }*)
-(*  destruct (strict_spec strict0 term); constructor. { constructor. exact Y. }*)
-(*  intros m C. invert C. apply N in strict_matched as [].*)
-(*Qed.*)
+Variant MoveOrReference (context : Context.context) : Pattern.move_or_reference -> Term.term -> Context.context -> Prop :=
+  | Mov strict term context_with_matches (S : Strict context strict term context_with_matches)
+      : MoveOrReference context (Pattern.Mov strict) term context_with_matches
+  | Ref
+      name term (lookup : Map.Find context name term)
+      strict old_context_with_matches cleaved (S : StrictRef context strict term cleaved old_context_with_matches)
+      context_with_matches (OW : Map.Overwrite name cleaved old_context_with_matches context_with_matches)
+      : MoveOrReference context (Pattern.Ref strict) (Term.Ref name) context_with_matches
+  .
+Arguments MoveOrReference context strict term context_with_matches.
+
+Example match_referenced_application ctor arg argn name (N : argn <> name)
+  : let pattern := Pattern.Ref (Pattern.App (Pattern.Ctr ctor) argn) in
+    let term := Term.App (Term.Ctr ctor) arg in
+    let context := Map.overriding_add name term Map.empty in
+    let context_with_matches :=
+      (* Note how each right-hand branch is turned into a `Mov` referencing the contents of the branch: *)
+      Map.overriding_add name (Term.App (Term.Ctr ctor) (Term.Mov argn)) (
+      Map.overriding_add argn arg (
+      Map.empty)) in
+    MoveOrReference context pattern (Term.Ref name) context_with_matches.
+Proof.
+  cbn. econstructor.
+  - apply Map.find_overriding_add. left. split; reflexivity.
+  - econstructor.
+    + constructor. intros x y. rewrite Map.find_singleton. rewrite Map.find_overriding_add.
+      split. { intros [[-> ->] | [N' F]]. { split; reflexivity. } invert F. }
+      intros [-> ->]. left. split; reflexivity.
+    + intro I. apply Map.in_singleton in I. apply N in I as [].
+    + apply Map.add_overriding. cbn. intros. apply Map.find_singleton in F as [Ea Ev]. apply N in Ea as [].
+  - split. { apply Map.in_overriding_add. right. apply Map.in_singleton. reflexivity. } split.
+    + intro F. apply Map.find_overriding_add in F as [[-> ->] | [N' F]]; [left | right]. { split; reflexivity. }
+      split. { exact N'. } apply Map.find_overriding_add.
+      apply Map.find_overriding_add in F as [[-> ->] | [N'' F]]; [left | right]. { split; reflexivity. }
+      split. { exact N''. } invert F.
+    + intro F. apply Map.find_overriding_add. destruct F as [[-> ->] | [N' F]]; [left | right]. { split; reflexivity. }
+      split. { exact N'. } apply Map.find_overriding_add.
+      apply Map.find_overriding_add in F as [[-> ->] | [N'' F]]. { left. split; reflexivity. }
+      apply Map.find_singleton in F as [E ->]. apply N' in E as [].
+Qed.
+
+Example match_referenced_application_deep ctor arg1 arg2 arg1n arg2n name
+  (N1 : arg1n <> name) (N2 : arg2n <> name) (N : arg2n <> arg1n)
+  : let pattern := Pattern.Ref (Pattern.App (Pattern.App (Pattern.Ctr ctor) arg1n) arg2n) in
+    let term := Term.App (Term.App (Term.Ctr ctor) arg1) arg2 in
+    let context := Map.overriding_add name term Map.empty in
+    let context_with_matches := (* Note how each right-hand branch is turned into a `Mov` referencing the contents of the branch: *)
+      Map.overriding_add name (Term.App (Term.App (Term.Ctr ctor) (Term.Mov arg1n)) (Term.Mov arg2n)) (
+      Map.overriding_add arg1n arg1 (
+      Map.overriding_add arg2n arg2 (
+      Map.empty))) in
+    MoveOrReference context pattern (Term.Ref name) context_with_matches.
+Proof.
+  cbn. econstructor.
+  - apply Map.find_overriding_add. left. split; reflexivity.
+  - econstructor.
+    + econstructor.
+      * constructor. intros x y. rewrite Map.find_singleton. rewrite Map.find_overriding_add.
+        split. { intros [[-> ->] | [N' F]]. { split; reflexivity. } invert F. }
+        intros [-> ->]. left. split; reflexivity.
+      * intro I. apply Map.in_singleton in I. apply N1 in I as [].
+      * apply Map.add_overriding. cbn. intros. apply Map.find_singleton in F as [Ea Ev]. apply N1 in Ea as [].
+    + intro I. apply Map.in_overriding_add in I as [E | I]. { apply N in E as []. }
+      apply Map.in_singleton in I. apply N2 in I as [].
+    + apply Map.add_overriding. cbn. intros.
+      apply Map.find_overriding_add in F as [[Ea Ev] | [N' F]]. { apply N in Ea as []. }
+      apply Map.find_singleton in F as [Ea Ev]. apply N2 in Ea as [].
+  - split. { apply Map.in_overriding_add. right. apply Map.in_overriding_add. right. apply Map.in_singleton. reflexivity. }
+    split.
+    + intro F. apply Map.find_overriding_add in F as [[-> ->] | [N' F]]; [left | right]. { split; reflexivity. }
+      split. { exact N'. } apply Map.find_overriding_add. rewrite Map.find_overriding_add.
+      apply Map.find_overriding_add in F as [[-> ->] | [N'' F]]. {
+        right. split. { symmetry. exact N. } left. split; reflexivity. }
+      apply Map.find_overriding_add in F as [[-> ->] | [N''' F]]; [left | right]. { split; reflexivity. } invert F.
+    + intro F. apply Map.find_overriding_add. destruct F as [[-> ->] | [N' F]]; [left | right]. { split; reflexivity. }
+      split. { exact N'. } apply Map.find_overriding_add. rewrite Map.find_overriding_add.
+      apply Map.find_overriding_add in F as [[-> ->] | [N'' F]]. { right. split. { exact N. } left. split; reflexivity. }
+      apply Map.find_overriding_add in F as [[-> ->] | [N''' F]]; [left | right]. { split; reflexivity. }
+      apply Map.find_singleton in F as [E ->]. apply N' in E as [].
+Qed.
+
+Definition move_or_reference context pattern term :=
+  match pattern with
+  | Pattern.Mov s => strict context s term
+  | Pattern.Ref s =>
+      match term with
+      | Term.Ref name =>
+          match Map.find context name with
+          | None => None
+          | Some term =>
+              match strict_ref context s term with
+              | None => None
+              | Some (cleaved, context_with_matches) =>
+                  Some (Map.overwrite name cleaved context_with_matches)
+              end
+          end
+      | _ => None
+      end
+  end.
+
+Lemma move_or_reference_det
+  c1 p1 t1 m1 (S1 : MoveOrReference c1 p1 t1 m1)
+  c2 (Ec : Map.Eq c1 c2)
+  p2 (Ep : p1 = p2)
+  t2 (Et : t1 = t2)
+  m2 (S2 : MoveOrReference c2 p2 t2 m2)
+  : Map.Eq m1 m2.
+Proof.
+  subst. invert S1; invert S2.
+  - eapply strict_det; try reflexivity; eassumption.
+  - apply Ec in lookup0. edestruct (Map.find_det lookup lookup0).
+    destruct (strict_ref_det S Ec eq_refl eq_refl S0) as [<- Eoc].
+    eapply Map.overwrite_det; try reflexivity; eassumption.
+Qed.
+
+Lemma in_move_or_reference {context move_or_reference term context_with_matches}
+  (MR : MoveOrReference context move_or_reference term context_with_matches) x
+  : Map.In context_with_matches x <-> (BoundIn.MoveOrReference move_or_reference x \/ Map.In context x).
+Proof.
+  invert MR.
+  - erewrite in_strict. 2: { exact S. } split; (intros [B | I]; [left | right; exact I]). { constructor. exact B. }
+    invert B. exact bound_in_strict.
+  - erewrite Map.in_overwrite. 2: { exact OW. } erewrite in_strict_ref. 2: { exact S. }
+    split; (intros [B | I]; [left | right; exact I]). { constructor. exact B. } invert B. exact bound_in_strict.
+Qed.
+
+Lemma move_or_reference_spec context pattern term
+  : Reflect.Option (MoveOrReference context pattern term) (move_or_reference context pattern term).
+Proof.
+  destruct pattern; cbn.
+  - cbn. destruct (strict_spec context strict0 term); constructor. { constructor. exact Y. }
+    intros x MR. invert MR. apply N in S as [].
+  - destruct term; try (constructor; intros m C; invert C).
+    destruct (Map.find_spec context name). 2: { constructor. intros m C. invert C. apply N in lookup as []. }
+    destruct (strict_ref_spec context strict0 x). 2: {
+      constructor. intros m C. invert C. destruct (Map.find_det Y lookup). apply (N (_, _)) in S as []. }
+    destruct x0 as [t ctx]; cbn in *. constructor. econstructor; try eassumption.
+    apply Map.overwrite_overwrite. eapply in_strict_ref. { exact Y0. } right. eexists. exact Y.
+Qed.
+
+
+
+Variant Pattern (context : Context.context) : Pattern.pattern -> Term.term -> Context.context -> Prop :=
+  | Nam
+      name (N : forall (I : Map.In context name), False)
+      term context_with_matches (S : Map.Add name term context context_with_matches)
+      : Pattern context (Pattern.Nam name) term context_with_matches
+  | Pat
+      move_or_reference term context_with_matches (move_or_reference_matched :
+        MoveOrReference context move_or_reference term context_with_matches)
+      : Pattern context (Pattern.Pat move_or_reference) term context_with_matches
+  .
+Arguments Pattern context pattern term context_with_matches.
+
+Definition pattern context patt term :=
+  match patt with
+  | Pattern.Nam name => Map.disjoint_add name term context
+  | Pattern.Pat mor => move_or_reference context mor term
+  end.
+
+Lemma pattern_det
+  c1 p1 t1 m1 (P1 : Pattern c1 p1 t1 m1)
+  c2 (Ec : Map.Eq c1 c2)
+  p2 (Ep : p1 = p2)
+  t2 (Et : t1 = t2)
+  m2 (P2 : Pattern c2 p2 t2 m2)
+  : Map.Eq m1 m2.
+Proof.
+  invert P1; invert P2.
+  - eapply Map.add_det; try reflexivity; eassumption.
+  - eapply move_or_reference_det; try reflexivity; eassumption.
+Qed.
+
+Lemma pattern_spec context patt term
+  : Reflect.Option (Pattern context patt term) (pattern context patt term).
+Proof.
+  destruct patt; cbn.
+  - destruct (Map.find_spec context name); constructor. { intros m C. invert C. apply N. eexists. exact Y. }
+    constructor. { intros [y F]. eapply N. exact F. } apply Map.add_overriding. cbn. intros. apply N in F as [].
+  - destruct (move_or_reference_spec context move_or_reference0 term); constructor. { constructor. exact Y. }
+    intros ctx C. invert C. apply N in move_or_reference_matched as [].
+Qed.
