theories/Context.v
@@ -1,0 +1,9 @@
+From LinearCore Require
+  Map
+  Term
+  .
+
+
+
+Definition context : Type := Map.to Term.term.
+Arguments context/.
